Working on AllRefs (unsure)

SafeBlocks.v
@@ -1,69 +1,195 @@
+From Coq Require Import Lia.
+
+From Elo Require Import Util.
+From Elo Require Import Map.
 From Elo Require Import Core.
 From Elo Require Import Access.
 From Elo Require Import UnsafeAccess.
 
+(* -------------------------------------------------------------------------- *)
+(* TODO                                                                       *)
+(* -------------------------------------------------------------------------- *)
+
+Inductive AllMutRefs (ad : addr) : tm -> Prop :=
+  | amr_unit :
+    AllMutRefs ad <{ unit }>
+
+  | amr_num : forall n,
+    AllMutRefs ad <{ N n }>
+
+  | amr_ref : forall T,
+    AllMutRefs ad <{ &ad :: &T }>
+
+  | amr_new : forall t T,
+    AllMutRefs ad t ->
+    AllMutRefs ad <{ new T t }>
+
+  | amr_load : forall t,
+    AllMutRefs ad t ->
+    AllMutRefs ad <{ *t }>
+
+  | amr_asg : forall t1 t2,
+    AllMutRefs ad t1 ->
+    AllMutRefs ad t2 ->
+    AllMutRefs ad <{ t1 = t2 }>
+
+  | amr_var : forall x,
+    AllMutRefs ad <{ var x }>
+
+  | amr_fun : forall t x Tx,
+    AllMutRefs ad t ->
+    AllMutRefs ad <{ fn x Tx --> t }>
+
+  | amr_call : forall t1 t2,
+    AllMutRefs ad t1 ->
+    AllMutRefs ad t2 ->
+    AllMutRefs ad <{ call t1 t2 }>
+    
+  | amr_seq : forall t1 t2,
+    AllMutRefs ad t1 ->
+    AllMutRefs ad t2 ->
+    AllMutRefs ad <{ t1; t2 }>
+
+  | amr_spawn : forall t,
+    AllMutRefs ad t ->
+    AllMutRefs ad <{ spawn t }>
+  .
+
+Inductive AllMutRefsMem (ad : addr) : mem -> Prop :=
+  | amrm_nil :
+    AllMutRefsMem ad nil
+
+  | amrm_cons_unit : forall m,
+    AllMutRefsMem ad m ->
+    AllMutRefsMem ad (cons <{ unit }> m)
+
+  | amrm_cons_num : forall m n,
+    AllMutRefsMem ad m ->
+    AllMutRefsMem ad (cons <{ N n }> m)
+
+  | amrm_cons_refI : forall m ad' T,
+    AllMutRefsMem ad m ->
+    ad <> ad' ->
+    AllMutRefsMem ad (cons <{ &ad' :: i&T }> m)
+
+  | amrm_cons_refM1 : forall m T ad',
+    AllMutRefsMem ad m ->
+    ad <> ad' ->
+    AllMutRefsMem ad (cons <{ &ad' :: &T }> m)
+
+  | amrm_cons_refM2 : forall m T,
+    AllMutRefsMem ad m ->
+    AllMutRefsMem ad (cons <{ &ad :: &T }> m)
+
+  | amrm_cons_fun : forall m t x Tx,
+    AllMutRefs ad t ->
+    AllMutRefsMem ad m ->
+    AllMutRefsMem ad (cons <{ fn x Tx --> t }> m)
+  .
+
+
+(* -------------------------------------------------------------------------- *)
+(* contains-block                                                             *)
+(* -------------------------------------------------------------------------- *)
+
 Reserved Notation " t 'contains_block' t' " (at level 30, no associativity).
 
-Inductive ContainsBlock (t' : tm) : tm -> Prop :=
-  | contains_block_new : forall t T,
+Inductive ContainsBlock : tm -> tm -> Prop :=
+  | contains_block_new : forall t t' T,
     t contains_block t' ->
     <{ new T t }> contains_block t'
 
-  | contains_block_load : forall t,
+  | contains_block_load : forall t t',
     t contains_block t' ->
     <{ *t }> contains_block t'
 
-  | contains_block_asg1 : forall t1 t2,
+  | contains_block_asg1 : forall t1 t2 t',
     t1 contains_block t' ->
     <{ t1 = t2 }> contains_block t'
 
-  | contains_block_asg2 : forall t1 t2,
+  | contains_block_asg2 : forall t1 t2 t',
     t2 contains_block t' ->
     <{ t1 = t2 }> contains_block t'
 
-  | contains_block_fun : forall t x Tx,
+  | contains_block_fun : forall t t' x Tx,
     t contains_block t' ->
     <{ fn x Tx --> t }> contains_block t'
 
-  | contains_block_call1 : forall t1 t2,
+  | contains_block_call1 : forall t1 t2 t',
     t1 contains_block t' ->
     <{ call t1 t2 }> contains_block t'
 
-  | contains_block_call2 : forall t1 t2,
+  | contains_block_call2 : forall t1 t2 t',
     t2 contains_block t' ->
     <{ call t1 t2 }> contains_block t'
 
-  | contains_block_seq1 : forall t1 t2,
+  | contains_block_seq1 : forall t1 t2 t',
     t1 contains_block t' ->
     <{ t1; t2 }> contains_block t'
 
-  | contains_block_seq2 : forall t1 t2,
+  | contains_block_seq2 : forall t1 t2 t',
     t2 contains_block t' ->
     <{ t1; t2 }> contains_block t'
 
-  | contains_block_spawn : forall t,
+  | contains_block_spawn : forall t t',
+    t <> t' ->
     t contains_block t' ->
     <{ spawn t }> contains_block t'
 
   | contains_block_eq : forall block,
-    block = t' ->
-    <{ spawn block }> contains_block t'
+    <{ spawn block }> contains_block block 
 
-  where "t 'contains_block' t'" := (ContainsBlock t' t).
-
-Lemma contains_block_trans : forall t1 t2 t3,
-  t1 contains_block t2 ->
-  t2 contains_block t3 ->
-  t1 contains_block t3.
-Proof.
-  intros * Hcon ?. induction Hcon; subst; eauto using ContainsBlock.
-Qed.
+  where "t 'contains_block' t'" := (ContainsBlock t t').
 
 Lemma step_spawn_contains_block : forall t t' block,
   t --[EF_Spawn block]--> t' ->
   t contains_block block.
 Proof.
   intros. induction_step; eauto using ContainsBlock.
+Qed.
+
+Lemma conblock_dec : forall t t',
+  Decidable.decidable (t contains_block t').
+Proof.
+  intros. induction t;
+  try solve [right; intros F; inversion F].
+  - destruct IHt.
+    + left. eauto using ContainsBlock.
+    + right. intros F. inversion F; subst. contradiction.
+  - destruct IHt.
+    + left. eauto using ContainsBlock.
+    + right. intros F. inversion F; subst. contradiction.
+  - destruct IHt1, IHt2.
+    + left. eauto using ContainsBlock.
+    + left. eauto using ContainsBlock.
+    + left. eauto using ContainsBlock.
+    + right. intros F. inversion F; subst; contradiction.
+  - destruct IHt.
+    + left. eauto using ContainsBlock.
+    + right. intros F. inversion F; subst. contradiction.
+  - destruct IHt1, IHt2.
+    + left. eauto using ContainsBlock.
+    + left. eauto using ContainsBlock.
+    + left. eauto using ContainsBlock.
+    + right. intros F. inversion F; subst; contradiction.
+  - destruct IHt1, IHt2.
+    + left. eauto using ContainsBlock.
+    + left. eauto using ContainsBlock.
+    + left. eauto using ContainsBlock.
+    + right. intros F. inversion F; subst; contradiction.
+  - destruct IHt.
+    + left. destruct (tm_eq_dec t t'); subst; eauto using ContainsBlock.
+    + right. intros F. inversion F; subst.
+      * contradiction.
+      * inversion F; subst.
+        ** contradiction.
+        ** admit.
+Abort.
+
+Lemma conblock_dec : forall t t',
+  Decidable.decidable (t contains_block t').
+Proof.
+  intros. eauto using classic_decidable.
 Qed.
 
 (* -------------------------------------------------------------------------- *)
@@ -75,4 +201,118 @@ Definition SafeBlocks (m : mem) (t : tm) := forall block ad,
   t contains_block block ->
   access m block ad ->
   ~ UnsafeAccess m t ad.
+
+(* -------------------------------------------------------------------------- *)
+(* constructor-sb                                                             *)
+(* -------------------------------------------------------------------------- *)
+
+Local Ltac solve_sb_con :=
+  intros * Hsb; intros ? ? ? H ? ?;
+  inversion_access; inversion_subst_clear H; inversion_uacc;
+  eapply Hsb; eauto.
+
+Local Lemma sb_con_new : forall m t T,
+  SafeBlocks m t ->
+  SafeBlocks m <{ new T t }>.
+Proof. solve_sb_con. Qed.
+
+Local Lemma sb_con_load : forall m t,
+  SafeBlocks m t ->
+  SafeBlocks m <{ *t }>.
+Proof. solve_sb_con. Qed.
+
+Local Lemma sb_con_asg: forall m t1 t2 T,
+  empty |-- t1 is <{{ & T }}> ->
+  empty |-- t2 is T ->
+  SafeBlocks m t1 ->
+  SafeBlocks m t2 ->
+  SafeBlocks m <{ t1 = t2 }>.
+Proof.
+  intros * Htype1 Htyp2 Hsb1 Hsb2. intros ? ? Hacc Hcon Hblock Huacc.
+  inversion_access; inversion_subst_clear Hcon; inversion_uacc;
+  try solve [eapply Hsb1; eauto];
+  try solve [eapply Hsb2; eauto].
+  - assert (access m t2 ad) by eauto using uacc_then_acc.
+    destruct (conblock_dec t2 block).
+    + specialize (Hsb2 block ad) as ?.
+      do 3 auto_specialize. contradiction.
+    + specialize (Hsb1 block ad H2 H3 Hblock) as ?.
+    
+    destruct (uacc_dec m t1 ad); try solve [eapply Hsb1; eauto].
+    eapply Hsb1; eauto.
+Abort.
+
+(* -------------------------------------------------------------------------- *)
+(* inversion-sb                                                               *)
+(* -------------------------------------------------------------------------- *)
+
+Local Ltac solve_inv_sb :=
+  intros * H; try split; intros ? ? ? ? ? ?;
+  eapply H; eauto using access, UnsafeAccess, ContainsBlock.
+
+Local Lemma sb_inv_new : forall m t T,
+  SafeBlocks m <{ new T t }> ->
+  SafeBlocks m t.
+Proof. solve_inv_sb. Qed.
+
+Local Lemma sb_inv_load : forall m t,
+  SafeBlocks m <{ *t }> ->
+  SafeBlocks m t.
+Proof. solve_inv_sb. Qed.
+
+Local Lemma sb_inv_asg : forall m t1 t2,
+  SafeBlocks m <{ t1 = t2 }> ->
+  (SafeBlocks m t1) /\ (SafeBlocks m t2).
+Proof. solve_inv_sb. Qed.
+
+Local Lemma sb_inv_fun : forall m t x Tx,
+  SafeBlocks m <{ fn x Tx --> t }> ->
+  SafeBlocks m t.
+Proof. solve_inv_sb. Qed.
+
+Local Lemma sb_inv_call : forall m t1 t2,
+  SafeBlocks m <{ call t1 t2 }> ->
+  (SafeBlocks m t1) /\ (SafeBlocks m t2).
+Proof. solve_inv_sb. Qed.
+
+Local Lemma sb_inv_seq : forall m t1 t2,
+  SafeBlocks m <{ t1; t2 }> ->
+  (SafeBlocks m t1) /\ (SafeBlocks m t2).
+Proof. solve_inv_sb. Qed.
+
+Ltac inversion_sb :=
+  match goal with
+  | H: SafeBlocks _ <{ new _ _      }> |- _ => eapply sb_inv_new  in H
+  | H: SafeBlocks _ <{ * _          }> |- _ => eapply sb_inv_load in H
+  | H: SafeBlocks _ <{ _ = _        }> |- _ => eapply sb_inv_asg  in H as [? ?]
+  | H: SafeBlocks _ <{ fn _ _ --> _ }> |- _ => eapply sb_inv_fun  in H
+  | H: SafeBlocks _ <{ call _ _     }> |- _ => eapply sb_inv_call in H as [? ?]
+  | H: SafeBlocks _ <{ _ ; _        }> |- _ => eapply sb_inv_seq  in H as [? ?]
+  end.
+
+(* -------------------------------------------------------------------------- *)
+(* safe-blocks-preservation                                                   *)
+(* -------------------------------------------------------------------------- *)
+
+Local Lemma step_none_sb_preservation : forall m t t' T,
+  empty |-- t is T ->
+  SafeBlocks m t ->
+  t --[EF_None]--> t' ->
+  SafeBlocks m t'.
+Proof.
+  intros. generalize dependent T.
+  induction_step; intros; inversion_type; inversion_sb;
+  eauto using sb_con_new, sb_con_load.
+  - do 2 auto_specialize. specialize (IHstep (<{{ &T0 }}>)). auto_specialize.
+    admit.
+  - admit.
+  - admit.
+  - admit.
+  - admit.
+  - admit.
+Qed.
+
+
+
+
 
